Make bvl_handle add split-markers into large BVL functions

compiler/backend/bvl_handleScript.sml
@@ -34,63 +34,70 @@ val LetLet_def = Define `
                                  | SOME k => Var k) env_length in
       Let (MAP Var zs) (SmartLet long_list body)`
 
+val OptionalLetLet_def = Define `
+  OptionalLetLet e env_size live s (limit:num) =
+    if s < limit then ([e],live,s) else
+      ([(Let [] (LetLet env_size live e))],live,0n)`;
+
 val compile_def = tDefine "compile" `
-  (compile n [] = ([]:bvl$exp list,Empty,0n)) /\
-  (compile n (x::y::xs) =
-     let (dx,lx,s1) = compile n [x] in
-     let (dy,ly,s2) = compile n (y::xs) in
+  (compile l n [] = ([]:bvl$exp list,Empty,0n)) /\
+  (compile l n (x::y::xs) =
+     let (dx,lx,s1) = compile l n [x] in
+     let (dy,ly,s2) = compile l n (y::xs) in
        (dx ++ dy, mk_Union lx ly, s1+s2)) /\
-  (compile n [Var v] = if v < n then ([Var v],Var v,1)
+  (compile l n [Var v] = if v < n then ([Var v],Var v,1)
                        else ([Op (Const 0) []],Empty,1)) /\
-  (compile n [If x1 x2 x3] =
-     let (x1,l1,s1) = compile n [x1] in
-     let (x2,l2,s2) = compile n [x2] in
-     let (x3,l3,s3) = compile n [x3] in
-       ([If (HD x1) (HD x2) (HD x3)],mk_Union l1 (mk_Union l2 l3),s1+s2+s3+1)) /\
-  (compile n [Let xs x2] =
+  (compile l n [If x1 x2 x3] =
+     let (x1,l1,s1) = compile l n [x1] in
+     let (x2,l2,s2) = compile l n [x2] in
+     let (x3,l3,s3) = compile l n [x3] in
+       OptionalLetLet (If (HD x1) (HD x2) (HD x3)) n
+         (mk_Union l1 (mk_Union l2 l3)) (s1+s2+s3+1) l) /\
+  (compile l n [Let xs x2] =
      if LENGTH xs = 0 then
-       compile n [x2]
+       compile l n [x2]
      else
        let k = LENGTH xs in
-       let (xs,l1,s1) = compile n xs in
-       let (x2,l2,s2) = compile (n + k) [x2] in
-         ([Let xs (HD x2)],mk_Union l1 (Shift k l2),s1+s2+1)) /\
-  (compile n [Handle x1 x2] =
-     let (y1,l1,s1) = compile n [x1] in
+       let (xs,l1,s1) = compile l n xs in
+       let (x2,l2,s2) = compile l (n + k) [x2] in
+         OptionalLetLet (Let xs (HD x2)) n
+           (mk_Union l1 (Shift k l2)) (s1+s2+1) l) /\
+  (compile l n [Handle x1 x2] =
+     let (y1,l1,s1) = compile l n [x1] in
        if no_raise y1 then (y1,l1,s1) else
-         let (y2,l2,s2) = compile (n+1) [x2] in
+         let (y2,l2,s2) = compile l (n+1) [x2] in
            ([Handle (LetLet n l1 (HD y1)) (HD y2)],
             mk_Union l1 (Shift 1 l2),
             s2 (* s1 intentionally left out because
                   it does not contrib to exp size in BVI *))) /\
-  (compile n [Raise x1] =
-     let (dx,lx,s1) = compile n [x1] in
-       ([Raise (HD dx)],lx,s1+1)) /\
-  (compile n [Op op xs] =
-     let (ys,l,s1) = compile n xs in
-       ([Op op ys],l,s1+1)) /\
-  (compile n [Tick x] =
-     let (y,l,s1) = compile n [x] in
-       ([Tick (HD y)],l,s1)) /\
-  (compile n [Call t dest xs] =
-     let (ys,l,s1) = compile n xs in
-       ([Call t dest ys],l,s1+1))`
- (WF_REL_TAC `measure (bvl$exp1_size o SND)`);
+  (compile l n [Raise x1] =
+     let (dx,lx,s1) = compile l n [x1] in
+       OptionalLetLet (Raise (HD dx)) n lx (s1+1) l) /\
+  (compile l n [Op op xs] =
+     let (ys,lx,s1) = compile l n xs in
+       OptionalLetLet (Op op ys) n lx (s1+1) l) /\
+  (compile l n [Tick x] =
+     let (y,lx,s1) = compile l n [x] in
+       ([Tick (HD y)],lx,s1)) /\
+  (compile l n [Call t dest xs] =
+     let (ys,lx,s1) = compile l n xs in
+       OptionalLetLet (Call t dest ys) n lx (s1+1) l)`
+ (WF_REL_TAC `measure (bvl$exp1_size o SND o SND)`);
 
 val compile_ind = theorem"compile_ind";
 
 val compile_exp_def = Define `
-  compile_exp arity e = HD (FST (compile arity [e]))`;
+  compile_exp arity e = HD (FST (compile 250 arity [e]))`;
 
 val compile_length = Q.store_thm("compile_length[simp]",
-  `!n xs. LENGTH (FST (compile n xs)) = LENGTH xs`,
+  `!l n xs. LENGTH (FST (compile l n xs)) = LENGTH xs`,
   HO_MATCH_MP_TAC compile_ind \\ REPEAT STRIP_TAC
   \\ fs [compile_def,ADD1,LET_DEF]
-  \\ rpt (pairarg_tac \\ fs []) \\ rw []);
+  \\ rpt (pairarg_tac \\ fs []) \\ rw [OptionalLetLet_def]);
 
 val compile_sing = store_thm("compile_sing",
-  ``compile n [x] = (dx,l,s) ==> ?y. dx = [y]``,
-  `LENGTH (FST (compile n [x])) = LENGTH [x]` by fs []
+  ``compile l n [x] = (dx,lx,s) ==> ?y. dx = [y]``,
+  `LENGTH (FST (compile l n [x])) = LENGTH [x]` by fs []
   \\ rpt strip_tac \\ full_simp_tac std_ss [LENGTH]
   \\ Cases_on `dx` \\ fs [LENGTH_NIL]);
 
